extraction/examples/BoardroomVotingExtraction.v
@@ -21,6 +21,7 @@ Open Scope Z.
 Definition PREFIX := "".
 
 From ConCert.Execution.Examples Require Import BoardroomVotingTest.
+Import Params.
 (* Get string representation of modulus, and remap it. This way we avoid having the extraction compute the number. *)
 Definition modulus_ := StringExtra.string_of_Z BoardroomVotingTest.modulus.
 
@@ -40,23 +41,50 @@ Print BoardroomMath.BoardroomAxioms.
     expeq := fun e e' : Z => e mod (order - 1) = e' mod (order - 
     order_ge_2 : order >
   ] *)
+Print Params.
+  Definition eqlemeqb_Z := @BoardroomMath.elmeqb _ Params.axioms.
+  
+  (* elmeq a b := a mod p = b mod p;
+     elmeqb a b := a mod p =? b mod p;
+     zero := 0;
+     one := 1;
+     add a a' := (a + a') mod p;
+     mul a a' := (a * a') mod p;
+     opp a := p - a;
+     inv a := Zp.mod_inv a p;
+     pow a e := Zp.mod_pow a e p;
+     order := p; *)
 
 (** A translation table for definitions we want to remap. The corresponding top-level definitions will be *ignored* *)
 Definition TT_remap : list (kername * string) :=
   TT_remap_default ++ [
-      remap <%% Amount %%> "tez"
-    ; remap <%% Z %%> "int"
-    ; remap <%% Z.add %%> "addInt"
-    ; remap <%% Z.sub %%> "subInt"
-    ; remap <%% Z.leb %%> "leInt"
-    ; remap <%% Z.ltb %%> "ltInt"
-    ; remap <%% Z.add %%> "addInt"
-    ; remap <%% Z.eqb %%> "eqInt"
-    ; remap <%% Z.gtb %%> "gtbInt"
-    ; remap <%% Nat.ltb %%> "ltbNat"
-    ; remap <%% Z.modulo %%> "modInt"
-    ; remap <%% Z.mul %%> "mulInt"
+    remap <%% Amount %%> "tez"
+  ;  remap <%% positive %%> "nat"
+  ; remap <%% Z %%> "int"
+  ; remap <%% Z.of_nat %%> "%int"
+  ; remap <%% Z.add %%> "addInt"
+  ; remap <%% Z.sub %%> "subInt"
+  ; remap <%% Z.leb %%> "leInt"
+  ; remap <%% Z.ltb %%> "ltInt"
+  ; remap <%% Z.add %%> "addInt"
+  ; remap <%% Z.eqb %%> "eqInt"
+  ; remap <%% Z.gtb %%> "gtbInt"
+  ; remap <%% Nat.ltb %%> "ltbNat"
+  ; remap <%% Z.modulo %%> "modInt"
+  ; remap <%% Z.mul %%> "mulInt"
+  ; remap <%% N.lxor %%> "xor"
+  ; remap <%% N.succ_pos %%> "(addNat 1)"
 
+  ; remap <%% BoardroomVotingTest.oneN %%> "1"
+  ; remap <%% BoardroomVotingTest.four %%> "4"
+  ; remap <%% BoardroomVotingTest.seven %%> "7"
+  ; remap <%% BoardroomVotingTest._1234583932 %%> "1234583932"
+  ; remap <%% BoardroomVotingTest._23241 %%> "23241"
+  ; remap <%% BoardroomVotingTest._159338231 %%> "159338231"
+  ; remap <%% BoardroomVotingTest._5 %%> "5"
+  ; remap <%% BoardroomVotingTest._3 %%> "3"
+  ; remap <%% BoardroomVotingTest._11 %%> "11"
+  ; remap <%% BoardroomVotingTest.five %%> "5"
   ; remap <%% @ContractCallContext %%> "(address * (address * int))"
   ; remap <%% @Chain %%> "(address * (address * address))" (* chain_height, current_slot, finalized_height *)
   ; remap <%% @chain_height %%> "fst" (* small hack, but valid since ContractCallContext is mapped to a tuple *)
@@ -71,6 +99,18 @@ Definition TT_remap : list (kername * string) :=
 
   ; remap <%% BoardroomMath.Zp.mod_pow %%> "mod_powInt"
   ; remap <%% BoardroomMath.Zp.mod_inv %%> "mod_invInt"
+  (*; remap <%% @BoardroomMath.add%%> "addInt"
+  ; remap <%% @BoardroomMath.elmeq%%> "eqInt"
+  ; remap <%% @BoardroomMath.expeq%%> "expeq"
+  ; remap <%% @BoardroomMath.elmeqb%%> "eqInt"
+  ; remap <%% @BoardroomMath.zero%%> "0"
+  ; remap <%% @BoardroomMath.one%%> "1"
+  ; remap <%% @BoardroomMath.mul%%> "mulInt"
+  ; remap <%% @BoardroomMath.opp%%> "-"
+  ; remap <%% @BoardroomMath.inv%%> "inv"
+  ; remap <%% @BoardroomMath.pow%%> "pow"
+  ; remap <%% @BoardroomMath.order%%> "order"
+  ; remap <%% @BoardroomVotingTest.axioms%%> "" *)
 
   (* ; remap <%% BV.verify_secret_vote_proof %%> "verify_secret_vote_proof" *)
   (* ; remap <%% @BV.make_signup_msg %%> "make_signup_msg" *)
@@ -79,26 +119,25 @@ Definition TT_remap : list (kername * string) :=
   (* ; remap <%% @BV.secret_vote_proof %%> "secret_vote_proof" *)
   (* ; remap <%% @BV.secret_key_proof %%> "secret_key_proof" *)
   (* ; remap <%% @BV.hash_sk_data %%> "hash_sk_data" *)
-  ; remap <%% @BV.hash_sv_data %%> "hash_sv_data"
+  (* ; remap <%% @BV.hash_sv_data %%> "hash_sv_data" *)
 
-  ; remap <%% @BV.handle_signup %%> "handle_signup"
+  (* ; remap <%% @BV.handle_signup %%> "handle_signup" *)
   ; remap <%% @BV.handle_commit_to_vote %%> "handle_commit_to_vote"
-  (* ; remap <%% @BV.handle_submit_vote %%> "handle_submit_vote" *)
-  (* ; remap <%% @BV.handle_tally_votes %%> "handle_tally_votes" *)
+  ; remap <%% @BV.handle_submit_vote %%> "handle_submit_vote"
+  ; remap <%% @BV.handle_tally_votes %%> "handle_tally_votes"
 
 
   ; remap <%% BoardroomVotingTest.modulus %%> modulus_
-
-  (* ; remap <%% @modulus_prime %%> "modulus_prime" *)
-  (* ; remap <%% @generator_is_generator %%> "generator_is_generator" *)
-  (* ; remap <%% @BoardroomMath.boardroom_axioms_Z %%> "BoardroomMath.boardroom_axioms_Z" *)
-  (* ; remap <%% @BoardroomMath.Generator %%> "BoardroomAxioms" *)
-  (* ; remap <%% @BoardroomMath.DiscreteLog %%> "BoardroomAxioms" *)
+  ; remap <%% @modulus_prime %%> "modulus_prime"
+  ; remap <%% BV.encodeA %%> "%nat"
+  ; remap <%% BV.encodeNat %%> "%nat"
   
 
-  ; remap <%% @List.map %%> "map"
-  ; remap <%% @List.find %%> "find"
-  ; remap <%% @countable.encode %%> "TODO_encode"
+  ; remap <%% @List.fold_left %%> "List.fold"
+  ; remap <%% @List.map %%> "List.map"
+  ; remap <%% @List.find %%> "List.find"
+  ; remap <%% @List.length %%> "List.length"
+  ; remap <%% @List.app %%> "List.append"
   ; remap <%% @Serializable.serialize %%> "TODO_serialize"
   ; remap <%% @Serializable.deserialize %%> "TODO_deserialize"
   ].
@@ -106,10 +145,17 @@ Definition TT_remap : list (kername * string) :=
 Definition TT_rename : list (string * string):=
   [ ("Some", "Some")
   ; ("None", "None")
+  ; ("Zpos" ,"%int")
+  ; ("Npos" ,"(fun (n:nat) -> n)")
+  ; ("Zneg" ,"-")
   ; ("Z0" ,"0")
+  ; ("N0" ,"0")
+  ; ("xH" ,"0")
+  ; ("1" ,"1")
   ; ("nil", "[]")
   ; ("true", "true")
   ; (string_of_kername <%% BV.State %%>, "State")  (* we add [storage] so it is printed without the prefix *) 
+  ; ("tt", "()")
   ].
 Require Import ContractMonads.
 
@@ -130,7 +176,7 @@ Definition receive_wrapper (msg : msg)
 Definition dummy_init : init_ctx -> BV.Setup -> option BV.State := fun _ _ => None .
 Definition dummy_receive : msg -> BV.State -> option (list ActionBody × BV.State) := 
   fun _ _  => 
-    let x := BoardroomMath.add 1 2 in
+    let x := BV.secret_key_proof 0 _5 five in
     None.
 
 Definition BV_MODULE : LiquidityMod msg init_ctx BV.Setup BV.State ActionBody :=
@@ -163,16 +209,27 @@ Definition inline_boardroom_params : list kername :=
       <%% Params.A %%>
     ; <%% Params.H %%>
     ; <%% Params.ser %%>
-    ; <%% Params.axioms %%>
+    (* ; <%% Params.axioms %%> *)
     ; <%% Params.gen %%>
     ; <%% Params.discr_log %%>
-    ; <%% BoardroomVotingTest.axioms_instance %%>
-    (* this *)
-    ; <%% BoardroomMath.boardroom_axioms_Z %%>
+    (* ; <%% BoardroomVotingTest.axioms_instance %%> *)
+    (* ; <%% BVZAxioms.boardroom_axioms_Z %%> *)
+
+    (* ; <%% @BoardroomMath.oeq_equivalence %%> *)
+    (* ; <%% @BoardroomMath.generator_instance %%> *)
+    (* ; <%% @BoardroomMath.generator %%> *)
+    (* ; <%% @BoardroomMath.generator_nonzero %%> *)
+    (* ; <%% @BoardroomMath.generator_generates %%> *)
+    (* ; <%% @BoardroomMath.log %%>
+    ; <%% @BoardroomMath.log_proper %%>
+    ; <%% @BoardroomMath.log_1_l %%>
+    ; <%% @BoardroomMath.log_generator %%> *)
 
     (* BoardroomAxioms *)
+    (* ; <%% @BoardroomMath.BoardroomAxioms%%>
     ; <%% @BoardroomMath.add%%>
-    (* ; <%% @BoardroomMath.elmeq%%> *)
+    ; <%% @BoardroomMath.elmeq%%>
+    ; <%% @BoardroomMath.expeq%%>
     ; <%% @BoardroomMath.elmeqb%%>
     ; <%% @BoardroomMath.zero%%>
     ; <%% @BoardroomMath.one%%>
@@ -180,8 +237,45 @@ Definition inline_boardroom_params : list kername :=
     ; <%% @BoardroomMath.opp%%>
     ; <%% @BoardroomMath.inv%%>
     ; <%% @BoardroomMath.pow%%>
-    ; <%% @BoardroomMath.order%%>
+    ; <%% @BoardroomMath.order%%> *)
 
+    (* ; <%% @BoardroomMath.plus_expeq_proper%%>
+    ; <%% @BoardroomMath.mul_expeq_proper%%>
+    ; <%% @BoardroomMath.sub_expeq_proper%%>
+    ; <%% @BoardroomMath.opp_expeq_proper%%>
+    ; <%% @BoardroomMath.pow_generator_proper%%>
+    ; <%% @BoardroomMath.prod_perm_proper%%>
+    ; <%% @BoardroomMath.bruteforce_tally_aux_proper%%>
+    ; <%% @BoardroomMath.bruteforce_tally_proper%%>
+    ; <%% @BoardroomMath.elmeqb_elmeq_proper%%>
+
+    ; <%% @BoardroomMath.elmeqb_spec%%>
+    ; <%% @BoardroomMath.order_ge_2%%>
+    ; <%% @BoardroomMath.elmeq_equiv%%>
+    ; <%% @BoardroomMath.add_proper%%>
+    ; <%% @BoardroomMath.mul_proper%%>
+    ; <%% @BoardroomMath.opp_proper%%>
+    ; <%% @BoardroomMath.inv_proper%%>
+    ; <%% @BoardroomMath.pow_base_proper%%>
+    ; <%% @BoardroomMath.pow_exp_proper%%>
+    ; <%% @BoardroomMath.one_neq_zero%%>
+    ; <%% @BoardroomMath.add_comm %%>
+    ; <%% @BoardroomMath.add_assoc %%>
+    ; <%% @BoardroomMath.mul_comm %%>
+    ; <%% @BoardroomMath.mul_assoc %%>
+    ; <%% @BoardroomMath.add_0_l %%>
+    ; <%% @BoardroomMath.mul_0_l %%>
+    ; <%% @BoardroomMath.mul_1_l %%>
+    ; <%% @BoardroomMath.opp_inv_l %%>
+    ; <%% @BoardroomMath.inv_inv_l %%>
+    ; <%% @BoardroomMath.mul_add %%>
+    ; <%% @BoardroomMath.pow_0_r %%>
+    ; <%% @BoardroomMath.pow_1_r %%>
+    ; <%% @BoardroomMath.pow_opp_1 %%>
+    ; <%% @BoardroomMath.pow_plus %%>
+    ; <%% @BoardroomMath.pow_pow %%>
+    ; <%% @BoardroomMath.pow_nonzero %%>
+    ; <%% @BoardroomMath.inv_nonzero %%> *)
   ].
 
 
@@ -253,7 +347,7 @@ Definition to_inline : list kername :=
   ; <%% @BV.set_VoterInfo_vote_hash %%>
   ; <%% @BV.set_VoterInfo_public_vote %%>
 
-
+  (* ; <%% @countable.encode %%> *)
   ].
 
 (* Definition asd := (BoardroomMath.add 1 2).
@@ -262,6 +356,11 @@ Time MetaCoq Quote Recursively Definition ex1 := asd.
 Check ex1.
 Definition r1 := Eval vm_compute in (liquidity_extract_single TT_remap TT_rename true BV_MODULE.(lmd_prelude) "harness?" ex1).
 Print r1. *)
+(* r1 = 
+inr
+  "Erased environment is not expanded enough for dearging to be provably correct"
+  : string + string
+*)
 
 Time MetaCoq Run
      (t <- liquidity_extraction_specialize PREFIX TT_remap TT_rename to_inline BV_MODULE ;;
@@ -271,4 +370,4 @@ Time MetaCoq Run
 Print liquidity_boardroomvoting.
 
 (** We redirect the extraction result for later processing and compiling with the Liquidity compiler *)
-Redirect "examples/liquidity-extract/CounterRefinementTypes.liq" Compute liquidity_counter.
+Redirect "examples/liquidity-extract/BoardroomVoting.liq" Compute liquidity_boardroomvoting.
